Add more changes

src/Syntax.v
@@ -19,7 +19,8 @@ Module Syntax (P : PAT).
   .
 
   Inductive type : Type :=
-  | TyVar  : tvar -> type
+  | TyBVar : tvar -> type
+  | TyFVar : tvar -> type
   | TyArr  : type -> type -> type
   | TyAll  : kind -> type -> type
   (* | TyProd : type -> type -> type *)
@@ -30,12 +31,13 @@ Module Syntax (P : PAT).
 
   #[export]
    Instance Inhab_type : Inhab type.
-  Proof. apply (Inhab_of_val (TyVar 0)). Qed.
+  Proof. apply (Inhab_of_val (TyFVar 0)). Qed.
 
   Inductive fin2 : Set := F1 | F2.
 
   Inductive term : Type :=
-  | TmVar    : var -> term
+  | TmBVar   : var -> term
+  | TmFVar   : var -> term
   | TmLam    : type -> term -> term
   | TmApp    : term -> term -> term
   | TmTyLam  : kind -> term -> term
@@ -55,64 +57,90 @@ Module Syntax (P : PAT).
 
   #[export]
    Instance Inhab_term : Inhab term.
-  Proof. apply (Inhab_of_val (TmVar 0)). Qed.
+  Proof. apply (Inhab_of_val (TmFVar 0)). Qed.
 
-  (* Shifting *)
-  (* X_shift_gen u i represents shifting all variables greater than or equal to i
-     in the term u by one. *)
 
-  Fixpoint ty_shift_gen (ty : type) (i : tvar) : type :=
+  (* Freshening *)
+  (* X_freshen u i represents an alpha-renaming making i fresh. *)
+
+  Fixpoint ty_freshen (ty : type) (i : tvar) : type :=
     match ty with
-    | TyVar j => (If i <= j then TyVar (S j) else ty)
-    | TyArr l r => TyArr (ty_shift_gen l i) (ty_shift_gen r i)
-    | TyAll k ty' => TyAll k (ty_shift_gen ty' (S i))
+    | TyBVar j => ty
+    | TyFVar k => If i <= k then TyFVar (S k) else ty
+    | TyArr l r => TyArr (ty_freshen l i) (ty_freshen r i)
+    | TyAll k ty' => TyAll k (ty_freshen ty' i)
     (* | TyProd l r => TyProd (ty_shift_gen l i) (ty_shift_gen r i) *)
     (* | TyCon ty' T => TyCon (ty_shift_gen ty' i) T *)
     (* | TySem l r ps => TySem (ty_shift_gen l i) (ty_shift_gen r i) ps *)
     (* | TyData d => ty *)
     end.
 
-  Definition ty_shift (ty : type) : type :=
-    ty_shift_gen ty 0.
-
-  Fixpoint tm_shift_gen (t : term) (i : var) : term :=
+  Fixpoint tm_freshen (t : term) (i : var) : term :=
     match t with
-    | TmVar j => (If i <= j then TmVar (S j) else t)
-    | TmLam ty t' => TmLam ty (tm_shift_gen t' (S i))
-    | TmApp l r => TmApp (tm_shift_gen l i) (tm_shift_gen r i)
-    | TmTyLam k t' => TmTyLam k (tm_shift_gen t' i)
-    | TmTyApp t' ty => TmTyApp (tm_shift_gen t' i) ty
+    | TmBVar j => t
+    | TmFVar k => If i <= k then TmFVar (S k) else t
+    | TmLam ty t' => TmLam ty (tm_freshen t' i)
+    | TmApp l r => TmApp (tm_freshen l i) (tm_freshen r i)
+    | TmTyLam k t' => TmTyLam k (tm_freshen t' i)
+    | TmTyApp t' ty => TmTyApp (tm_freshen t' i) ty
     end.
 
-  Definition tm_shift (t : term) : term :=
-    tm_shift_gen t 0.
-
-  Fixpoint tm_ty_shift_gen (t : term) (i : tvar) : term :=
+  Fixpoint tm_ty_freshen (t : term) (i : tvar) : term :=
     match t with
-    | TmVar j => t
-    | TmLam ty t' => TmLam (ty_shift_gen ty i) (tm_ty_shift_gen t' i)
-    | TmApp l r => TmApp (tm_ty_shift_gen l i) (tm_ty_shift_gen r i)
-    | TmTyLam k t' => TmTyLam k (tm_ty_shift_gen t' (S i))
-    | TmTyApp t' ty => TmTyApp (tm_ty_shift_gen t' i) (ty_shift_gen ty i)
+    | TmBVar j => t
+    | TmFVar k => t
+    | TmLam ty t' => TmLam (ty_freshen ty i) (tm_ty_freshen t' i)
+    | TmApp l r => TmApp (tm_ty_freshen l i) (tm_ty_freshen r i)
+    | TmTyLam k t' => TmTyLam k (tm_ty_freshen t' i)
+    | TmTyApp t' ty => TmTyApp (tm_ty_freshen t' i) (ty_freshen ty i)
     end.
 
-  Fixpoint tm_ty_shift (t : term) : term :=
-    tm_ty_shift_gen t 0.
+  (* Defreshening *)
+  (* X_defreshen u i represents an alpha-renaming making i occupied. *)
 
+  Fixpoint ty_defreshen (ty : type) (i : tvar) : type :=
+    match ty with
+    | TyBVar j => ty
+    | TyFVar k => If i <= k then TyFVar (k - 1) else ty
+    | TyArr l r => TyArr (ty_defreshen l i) (ty_defreshen r i)
+    | TyAll k ty' => TyAll k (ty_defreshen ty' i)
+    (* | TyProd l r => TyProd (ty_shift_gen l i) (ty_shift_gen r i) *)
+    (* | TyCon ty' T => TyCon (ty_shift_gen ty' i) T *)
+    (* | TySem l r ps => TySem (ty_shift_gen l i) (ty_shift_gen r i) ps *)
+    (* | TyData d => ty *)
+    end.
 
-  (* Substitution *)
-  (* X_subst_gen u i v represents the term u[i \mapsto v] *)
+  Fixpoint tm_defreshen (t : term) (i : var) : term :=
+    match t with
+    | TmBVar j => t
+    | TmFVar k => If i <= k then TmFVar (k - 1) else t
+    | TmLam ty t' => TmLam ty (tm_defreshen t' i)
+    | TmApp l r => TmApp (tm_defreshen l i) (tm_defreshen r i)
+    | TmTyLam k t' => TmTyLam k (tm_defreshen t' i)
+    | TmTyApp t' ty => TmTyApp (tm_defreshen t' i) ty
+    end.
 
-  Fixpoint ty_subst_gen (ty1 : type) (i : tvar) (ty2 : type) : type :=
+  Fixpoint tm_ty_defreshen (t : term) (i : tvar) : term :=
+    match t with
+    | TmBVar j => t
+    | TmFVar k => t
+    | TmLam ty t' => TmLam (ty_defreshen ty i) (tm_ty_defreshen t' i)
+    | TmApp l r => TmApp (tm_ty_defreshen l i) (tm_ty_defreshen r i)
+    | TmTyLam k t' => TmTyLam k (tm_ty_defreshen t' i)
+    | TmTyApp t' ty => TmTyApp (tm_ty_defreshen t' i) (ty_defreshen ty i)
+    end.
+
+  (* Bound variable substitution *)
+  (* X_bsubst u i v represents the substitution u[i \mapsto v], where i is bound in u. *)
+
+  Fixpoint ty_bsubst (ty1 : type) (i : tvar) (ty2 : type) : type :=
     match ty1 with
-    | TyVar j =>
-        (If j < i then TyVar j else
-           If j = i then ty2 else
-           TyVar (j - 1))
+    | TyBVar j => If j = i then ty2 else ty1
+    | TyFVar k => ty1
     | TyArr l r =>
-        TyArr (ty_subst_gen l i ty2) (ty_subst_gen r i ty2)
+        TyArr (ty_bsubst l i ty2) (ty_bsubst r i ty2)
     | TyAll k ty1' =>
-        TyAll k (ty_subst_gen ty1' (S i) (ty_shift ty2))
+        TyAll k (ty_bsubst ty1' (S i) ty2)
     (* | TyProd l r => *)
     (*     TyProd (ty_subst_gen l i ty2) (ty_subst_gen r i ty2) *)
     (* | TyCon ty1' T => *)
@@ -122,37 +150,75 @@ Module Syntax (P : PAT).
     (* | TyData d => ty1 *)
     end.
 
-  Definition ty_subst (ty1 : type) (ty2 : type) : type :=
-    ty_subst_gen ty1 0 ty2.
-
-  Fixpoint tm_subst_gen (t1 : term) (i : var) (t2 : term) : term :=
+  Fixpoint tm_bsubst (t1 : term) (i : var) (t2 : term) : term :=
     match t1 with
-    | TmVar j =>
-        (If j < i then TmVar j else
-           If j = i then t2 else
-           TmVar (j - 1))
-    | TmLam ty t1' => TmLam ty (tm_subst_gen t1' (S i) (tm_shift t2))
-    | TmApp l r => TmApp (tm_subst_gen l i t2) (tm_subst_gen r i t2)
-    | TmTyLam k t1' => TmTyLam k (tm_subst_gen t1' i (tm_ty_shift t2))
-    | TmTyApp t1' ty => TmTyApp (tm_subst_gen t1' i t2) ty
+    | TmBVar j => If j = i then t2 else t1
+    | TmFVar k => t1
+    | TmLam ty t1' => TmLam ty (tm_bsubst t1' (S i) t2)
+    | TmApp l r => TmApp (tm_bsubst l i t2) (tm_bsubst r i t2)
+    | TmTyLam k t1' => TmTyLam k (tm_bsubst t1' i t2)
+    | TmTyApp t1' ty => TmTyApp (tm_bsubst t1' i t2) ty
     end.
 
-  Definition tm_subst (t1 : term) (t2 : term) : term :=
-    tm_subst_gen t1 0 t2.
-
-  Fixpoint tm_ty_subst_gen (t : term) (i : tvar) (ty : type) : term :=
+  Fixpoint tm_ty_bsubst (t : term) (i : tvar) (ty : type) : term :=
     match t with
-    | TmVar j => t
-    | TmLam ty' t' => TmLam (ty_subst_gen ty' i ty) (tm_ty_subst_gen t' i ty)
-    | TmApp l r => TmApp (tm_ty_subst_gen l i ty) (tm_ty_subst_gen r i ty)
-    | TmTyLam k t' => TmTyLam k (tm_ty_subst_gen t' (S i) ty)
-    | TmTyApp t' ty' => TmTyApp (tm_ty_subst_gen t' i ty) (ty_subst_gen ty' i ty)
+    | TmBVar j => t
+    | TmFVar k => t
+    | TmLam ty' t' => TmLam (ty_bsubst ty' i ty) (tm_ty_bsubst t' i ty)
+    | TmApp l r => TmApp (tm_ty_bsubst l i ty) (tm_ty_bsubst r i ty)
+    | TmTyLam k t' => TmTyLam k (tm_ty_bsubst t' (S i) ty)
+    | TmTyApp t' ty' => TmTyApp (tm_ty_bsubst t' i ty) (ty_bsubst ty' i ty)
     end.
 
-  Definition tm_ty_subst (t : term) (ty : type) : term :=
-    tm_ty_subst_gen t 0 ty.
+  (* Free variable substitution *)
+  Fixpoint ty_subst (ty1 : type) (i : tvar) (ty2 : type) : type :=
+    match ty1 with
+    | TyBVar j => ty1
+    | TyFVar k => If k = i then ty2 else ty1
+    | TyArr l r =>
+        TyArr (ty_subst l i ty2) (ty_subst r i ty2)
+    | TyAll k ty1' =>
+        TyAll k (ty_subst ty1' i ty2)
+    (* | TyProd l r => *)
+    (*     TyProd (ty_subst_gen l i ty2) (ty_subst_gen r i ty2) *)
+    (* | TyCon ty1' T => *)
+    (*     TyCon (ty_subst_gen ty1' i ty2) T *)
+    (* | TySem l r ps => *)
+    (*     TySem (ty_subst_gen l i ty2) (ty_subst_gen r i ty2) ps *)
+    (* | TyData d => ty1 *)
+    end.
 
-  Definition tm_subst_n (t : term) (ts : list term) : term :=
-    fold_right (fun t2 t1 => tm_subst t1 t2) t ts.
+  Fixpoint tm_subst (t1 : term) (i : var) (t2 : term) : term :=
+    match t1 with
+    | TmBVar j => t1
+    | TmFVar k => If k = i then t2 else t1
+    | TmLam ty t1' => TmLam ty (tm_subst t1' i t2)
+    | TmApp l r => TmApp (tm_subst l i t2) (tm_subst r i t2)
+    | TmTyLam k t1' => TmTyLam k (tm_subst t1' i t2)
+    | TmTyApp t1' ty => TmTyApp (tm_subst t1' i t2) ty
+    end.
+
+  Fixpoint tm_ty_subst (t : term) (i : tvar) (ty : type) : term :=
+    match t with
+    | TmBVar j => t
+    | TmFVar k => t
+    | TmLam ty' t' => TmLam (ty_subst ty' i ty) (tm_ty_subst t' i ty)
+    | TmApp l r => TmApp (tm_ty_subst l i ty) (tm_ty_subst r i ty)
+    | TmTyLam k t' => TmTyLam k (tm_ty_subst t' i ty)
+    | TmTyApp t' ty' => TmTyApp (tm_ty_subst t' i ty) (ty_subst ty' i ty)
+    end.
+
+  (* Opening *)
+  Definition ty_open (ty : type) : type := ty_bsubst (ty_freshen ty 0) 0 (TyFVar 0).
+  Definition tm_open (t : term) : term := tm_bsubst (tm_freshen t 0) 0 (TmFVar 0).
+  Definition tm_ty_open (t : term) : term := tm_ty_bsubst (tm_ty_freshen t 0) 0 (TyFVar 0).
+
+  (* Closing *)
+  Definition ty_close (ty : type) : type := ty_defreshen (ty_subst ty 0 (TyBVar 0)) 0.
+  Definition tm_close (t : term) : term := tm_defreshen (tm_subst t 0 (TmBVar 0)) 0.
+  Definition tm_ty_close (t : term) : term := tm_ty_defreshen (tm_ty_subst t 0 (TyBVar 0)) 0.
+
+  (* Definition tm_subst_n (t : term) (ts : list term) : term := *)
+  (*   fold_right (fun t2 t1 => tm_subst t1 t2) t ts. *)
 
 End Syntax.
