src/Env.v
@@ -1,4 +1,4 @@
-From MCore Require Import Syntax.
+From MCore Require Import Syntax Tactics.
 From TLC Require Import LibList.
 Import LibListNotation.
 
@@ -12,41 +12,66 @@ Module Env (P : PAT).
   .
 
   Inductive binding : Type :=
-  | BTname : binding
-  | Bcon   : data -> type -> tname -> binding
-  | Btvar  : kind -> binding
-  | Bvar   : type -> binding
-  | Bmatch : match_assum -> binding
+  | BindTname : binding
+  | BindCon   : data -> type -> tname -> binding
+  | BindTvar  : kind -> binding
+  | BindVar   : option type -> binding
+  | BindMatch : match_assum -> binding
   .
 
   Definition env : Type := list binding.
 
-  Definition is_tname (b : binding) : Prop := match b with BTname => True | _ => False end.
+  Definition is_tname (b : binding) : Prop := match b with BindTname => True | _ => False end.
   Definition tnames   (Gamma : env) : env := filter is_tname Gamma.
 
-  Definition is_con (b : binding) : Prop := match b with Bcon _ _ _ => True | _ => False end.
+  Definition is_con (b : binding) : Prop := match b with BindCon _ _ _ => True | _ => False end.
   Definition cons   (Gamma : env) : env := filter is_con Gamma.
 
-  Definition is_tvar (b : binding) : Prop := match b with Btvar _ => True | _ => False end.
+  Definition is_tvar (b : binding) : Prop := match b with BindTvar _ => True | _ => False end.
   Definition tvars   (Gamma : env) : env := filter is_tvar Gamma.
 
-  Definition is_var (b : binding) : Prop := match b with Bvar _ => True | _ => False end.
+  Definition is_var (b : binding) : Prop := match b with BindVar _ => True | _ => False end.
   Definition vars   (Gamma : env) : env := filter is_var Gamma.
 
-  Definition is_match (b : binding) : Prop := match b with Bmatch _ => True | _ => False end.
-  Definition matches (Gamma : env) : env := filter is_match Gamma.
+  Definition is_match (b : binding) : Prop := match b with BindMatch _ => True | _ => False end.
+  Definition matches  (Gamma : env) : env := filter is_match Gamma.
 
   Definition tname_in (T : tname) (Gamma : env) : Prop :=
-    Nth T Gamma BTname.
+    Nth T Gamma BindTname.
 
   Definition con_in (K : con) (d : data) (ty : type) (T : tname) (Gamma : env) : Prop :=
-    Nth K Gamma (Bcon d ty T).
+    Nth K Gamma (BindCon d ty T).
 
   Definition tvar_in (tv : tvar) (k : kind) (Gamma : env) : Prop :=
-    Nth tv Gamma (Btvar k).
+    Nth tv Gamma (BindTvar k).
 
-  Definition var_in (v : var) (ty : type) (Gamma : env) : Prop :=
-    Nth v Gamma (Bvar ty).
+  Definition var_in (v : var) (ty : option type) (Gamma : env) : Prop :=
+    Nth v Gamma (BindVar ty).
 
   Definition empty_env : env := [ ].
+
+
+
+  Lemma vars_app : forall G1 G2, vars (G1 ++ G2) = vars G1 ++ vars G2.
+  Proof. intros. unfold vars. rew_listx~. Qed.
+
+  Lemma vars_cons : forall Gamma b,
+      vars (b :: Gamma) =
+        match b with
+        | BindVar _ => b :: vars Gamma
+        | _         => vars Gamma
+        end.
+  Proof. intros ; destruct b ; unfold vars ; rew_listx ; rew_mcore~. Qed.
+
+  #[export]
+  Hint Rewrite vars_app vars_cons : rew_mcore.
+
+  (* Lemma var_in_n : forall G1 G2 b, *)
+  (*     var_in (length G1) (G1 ++ b ++ G2) = *)
+  (*       match b with *)
+  (*       | BindVar _ => b :: vars Gamma *)
+  (*       | _         => vars Gamma *)
+  (*       end. *)
+  (* Proof. intros ; destruct b ; unfold vars ; rew_listx ; rew_mcore~. Qed. *)
+
 End Env.
