src/Soundness.v
@@ -7,20 +7,6 @@ Module Soundness (P : PAT).
   Module S := SmallStep P.
   Import S.
 
-  Ltac auto_star ::=
-    unfolds tvars ;
-    unfolds tvar_in ;
-    unfolds is_tvar ;
-    unfolds vars ;
-    unfolds var_in ;
-    unfolds is_var ;
-    try (rewrites (>> If_l True) in *) ;
-    try (rewrites (>> If_r False) in *) ;
-    rew_listx in *;
-    try solve [ auto with mcore
-              | eauto with mcore
-              | intuition eauto with mcore].
-
   Module Soundness (PC : PATCHECK) (M : MATCH).
     Module Typing := Typing PC.
     Module SmallStep := SmallStep M.
@@ -35,7 +21,7 @@ Module Soundness (P : PAT).
       remember empty_env as Gamma eqn:HGamma.
       induction ttype
       ; try (left; constructor).
-      { Case "TmVar". subst. with_hyp (var_in _ _ _) as H. inversion H. }
+      { Case "TmFVar". subst. with_hyp (var_in _ _ _) as H. inversion H. }
       { Case "TmApp". right.
         forwards* [Hval1 | (t1' & Hstep1)]: IHttype1.
         forwards* [Hval2 | (t2' & Hstep2)]: IHttype2.
@@ -45,56 +31,56 @@ Module Soundness (P : PAT).
         inverts* Hval. inverts ttype. }
     Qed.
 
-    Lemma ok_kind_strengthen_vars :
-      forall G1 G2 ty' k,
-        ok_kind (G1 ++ Bvar ty' :: G2) k ->
-        ok_kind (G1 ++ G2) k.
-    Proof. introv k_wf. induction* k_wf. Qed.
+    (* Lemma ok_kind_strengthen_vars : *)
+    (*   forall G1 G2 ty' k, *)
+    (*     ok_kind (G1 ++ Bvar ty' :: G2) k -> *)
+    (*     ok_kind (G1 ++ G2) k. *)
+    (* Proof. introv k_wf. induction* k_wf. Qed. *)
 
-    Lemma ok_kind_strengthen_tvars :
-      forall G1 G2 k' k,
-        ok_kind (G1 ++ G2) k ->
-        ok_kind (G1 ++ Btvar k' :: G2) k.
-    Proof. introv k_wf. induction* k_wf. Qed.
+    (* Lemma ok_kind_strengthen_tvars : *)
+    (*   forall G1 G2 k' k, *)
+    (*     ok_kind (G1 ++ G2) k -> *)
+    (*     ok_kind (G1 ++ Btvar k' :: G2) k. *)
+    (* Proof. introv k_wf. induction* k_wf. Qed. *)
 
-    Lemma ok_type_strengthen_vars :
-      forall G1 G2 ty' ty k,
-        ok_type (G1 ++ Bvar ty' :: G2) ty k ->
-        ok_type (G1 ++ G2) ty k.
-    Proof.
-      introv tykind.
-      remember (G1 ++ Bvar ty' :: G2) as Gamma eqn:HGamma.
-      gen G1.
-      induction tykind ; intros ; subst* ; constructor*.
-      { Case "TyAll". applys* IHtykind (Btvar k :: G1). }
-    Qed.
+    (* Lemma ok_type_strengthen_vars : *)
+    (*   forall G1 G2 ty' ty k, *)
+    (*     ok_type (G1 ++ Bvar ty' :: G2) ty k -> *)
+    (*     ok_type (G1 ++ G2) ty k. *)
+    (* Proof. *)
+    (*   introv tykind. *)
+    (*   remember (G1 ++ Bvar ty' :: G2) as Gamma eqn:HGamma. *)
+    (*   gen G1. *)
+    (*   induction tykind ; intros ; subst* ; constructor*. *)
+    (*   { Case "TyAll". applys* IHtykind (Btvar k :: G1). } *)
+    (* Qed. *)
 
-    Definition ty_shift_env Gamma :=
-      fold_right
-        (fun b bs =>
-           match b with
-           | Bvar ty => Bvar (ty_shift_gen ty (length (tvars bs)))
-           | _ => b
-           end :: bs)
-        [ ] Gamma.
+    (* Definition ty_shift_env Gamma := *)
+    (*   fold_right *)
+    (*     (fun b bs => *)
+    (*        match b with *)
+    (*        | Bvar ty => Bvar (ty_shift_gen ty (length (tvars bs))) *)
+    (*        | _ => b *)
+    (*        end :: bs) *)
+    (*     [ ] Gamma. *)
 
-    Lemma ty_shift_env_length :
-      forall Gamma,
-        length (tvars (ty_shift_env Gamma)) = length (tvars Gamma).
-    Proof. Admitted.
+    (* Lemma ty_shift_env_length : *)
+    (*   forall Gamma, *)
+    (*     length (tvars (ty_shift_env Gamma)) = length (tvars Gamma). *)
+    (* Proof. Admitted. *)
 
-    Lemma ok_kind_strengthen_shift :
-      forall G1 G2 k,
-        ok_kind (G1 ++ G2) k ->
-        ok_kind (ty_shift_env G1 ++ G2) k.
-    Proof. Admitted.
+    (* Lemma ok_kind_strengthen_shift : *)
+    (*   forall G1 G2 k, *)
+    (*     ok_kind (G1 ++ G2) k -> *)
+    (*     ok_kind (ty_shift_env G1 ++ G2) k. *)
+    (* Proof. Admitted. *)
 
 
-    Lemma ok_type_weaken_tvars_gen :
-      forall G1 G2 k' ty k,
-        ok_type (G1 ++ G2) ty k ->
-        ok_type (ty_shift_env G1 ++ k' :: G2) (ty_shift_gen ty (length (tvars G1))) k.
-    Proof. Admitted.
+    (* Lemma ok_type_weaken_tvars_gen : *)
+    (*   forall G1 G2 k' ty k, *)
+    (*     ok_type (G1 ++ G2) ty k -> *)
+    (*     ok_type (ty_shift_env G1 ++ k' :: G2) (ty_shift_gen ty (length (tvars G1))) k. *)
+    (* Proof. Admitted. *)
 
     (* Lemma ok_type_tvars_weaken : *)
     (*   forall Gamma k' ty k, *)
@@ -105,29 +91,29 @@ Module Soundness (P : PAT).
     (* Lemma shift_subst_comm : *)
     (*   forall t1  *)
 
-    Lemma ok_term_weaken_tvars_gen :
-      forall G1 G2 k t ty,
-        ok_term (G1 ++ G2) t ty ->
-        ok_term (ty_shift_env G1 ++ Btvar k :: G2)
-                (tm_ty_shift_gen t (length (tvars G1)))
-                (ty_shift_gen ty (length (tvars G1))).
-    Proof.
-      introv ttype.
-      remember (G1 ++ G2) as Gamma eqn:HGamma.
-      gen G1.
-      induction ttype ; intros ; subst*.
-      { Case "TmVar". admit. }
-      { Case "TmLam". constructor.
-        applys* ok_type_weaken_tvars_gen.
-        applys_eq* (IHttype (Bvar ty1 :: G1)). unfolds* ty_shift_env. rewrite* ty_shift_env_length.
-        auto_star. auto_star. }
-      { Case "TmTyLam". constructor.
-        applys ok_kind_strengthen_tvars.
-        applys* ok_kind_strengthen_shift.
-        applys_eq* (IHttype (Btvar k0 :: G1)) ; rew_listx*. }
-      { Case "TmTyApp". unfold ty_shift_gen.  constructor.
-      }
-    Admitted.
+    (* Lemma ok_term_weaken_tvars_gen : *)
+    (*   forall G1 G2 k t ty, *)
+    (*     ok_term (G1 ++ G2) t ty -> *)
+    (*     ok_term (ty_shift_env G1 ++ Btvar k :: G2) *)
+    (*             (tm_ty_shift_gen t (length (tvars G1))) *)
+    (*             (ty_shift_gen ty (length (tvars G1))). *)
+    (* Proof. *)
+    (*   introv ttype. *)
+    (*   remember (G1 ++ G2) as Gamma eqn:HGamma. *)
+    (*   gen G1. *)
+    (*   induction ttype ; intros ; subst*. *)
+    (*   { Case "TmVar". admit. } *)
+    (*   { Case "TmLam". constructor. *)
+    (*     applys* ok_type_weaken_tvars_gen. *)
+    (*     applys_eq* (IHttype (Bvar ty1 :: G1)). unfolds* ty_shift_env. rewrite* ty_shift_env_length. *)
+    (*     auto_star. auto_star. } *)
+    (*   { Case "TmTyLam". constructor. *)
+    (*     applys ok_kind_strengthen_tvars. *)
+    (*     applys* ok_kind_strengthen_shift. *)
+    (*     applys_eq* (IHttype (Btvar k0 :: G1)) ; rew_listx*. } *)
+    (*   { Case "TmTyApp". unfold ty_shift_gen.  constructor. *)
+    (*   } *)
+    (* Admitted. *)
 
     (* Lemma ok_term_tvars_weaken : *)
     (*   forall Gamma k t ty, *)
@@ -135,58 +121,92 @@ Module Soundness (P : PAT).
     (*     ok_term (Gamma <| tvars ::= fun tvs => k :: tvs |>) (tm_ty_shift t) (ty_shift ty). *)
     (* Proof. Admitted. *)
 
-    Lemma ok_term_weaken_vars :
-      forall Gamma ty' t ty,
+    (* Lemma ok_term_weaken_vars : *)
+    (*   forall Gamma ty' t ty, *)
+    (*     ok_term Gamma t ty -> *)
+    (*     ok_term (Bvar ty' :: Gamma) (tm_shift t) ty. *)
+    (* Proof. Admitted. *)
+
+    (* Lemma tm_subst_gen_preservation : *)
+    (*   forall G1 G2 t ty t' ty', *)
+    (*     ok_term (G1 ++ Bvar ty' :: G2) t ty -> *)
+    (*     ok_term (G1 ++ G2) t' ty' -> *)
+    (*     ok_term (G1 ++ G2) (tm_subst_gen t (length (vars G1)) t') ty. *)
+    (* Proof. *)
+    (*   introv ttype. *)
+    (*   remember (G1 ++ Bvar ty1 :: G2) as Gamma eqn:HGamma. *)
+    (*   gen t' ty1 G1. *)
+    (*   induction ttype ; intros ; subst*. *)
+    (*   { Case "TmVar". with_hyp (Nth _ _ _) as Hvar. *)
+    (*     unfold tm_subst_gen. *)
+    (*     lets [ in_vs1 | (m & Heqm & in_vs2') ] : Nth_app_inv Hvar. *)
+    (*     { lets Hlt : Nth_inbound in_vs1. rewrites (>> If_l Hlt). *)
+    (*       constructor*. applys* Nth_app_l. } *)
+    (*     { subst. assert (nlt : ~(length (vars G1) + m < length (vars G1))). nat_math. *)
+    (*       rewrites* (>> If_r nlt). *)
+    (*       lets [ (Heq0 & Heq) | (m' & Heqm' & in_vs2) ] : Nth_cons_inv in_vs2' ; subst. *)
+    (*       { inverts Heq. rewrites* (>> If_l plus_zero_r). } *)
+    (*       { rew_nat. assert (neq : S (length (vars G1) + m') <> length (vars G1)). nat_math. *)
+    (*         rewrites (>> If_r neq). rewrite Nat.add_comm. *)
+    (*         constructor*. applys Nth_app_r in_vs2. } } } *)
+    (*   { Case "TmLam". constructors*. *)
+    (*     applys* ok_type_strengthen_vars ty0. *)
+    (*     applys_eq* (IHttype (tm_shift t') ty0 (Bvar ty1 :: G1)). unfolds* is_var. *)
+    (*     applys_eq* (ok_term_weaken_vars (G1 ++ G2) ty1). } *)
+    (*   { Case "TmTyLam". constructors*. *)
+    (*     applys* ok_kind_strengthen_vars ty1. folds (tm_subst_gen t (length (filter is_var G1)) (tm_ty_shift t')). *)
+    (*     applys_eq* (IHttype (tm_ty_shift t') (Btvar k :: G1) (ty_shift ty1)). *)
+    (*     applys* ok_term_tvars_weaken (Gamma <| vars := vs1 ++ vs2 |> <| tvars := tvs |>). } *)
+    (*   { Case "TmTyApp". constructors*. *)
+    (*     applys* ok_type_ignores_vars (Gamma <| vars := vs1 ++ ty1 :: vs2 |> <| tvars := tvs |>). } *)
+    (* Qed. *)
+
+    Lemma tm_freshen_preservation :
+      forall Gamma t ty ty',
         ok_term Gamma t ty ->
-        ok_term (Bvar ty' :: Gamma) (tm_shift t) ty.
+        ok_term (BindVar ty' :: Gamma) (tm_freshen t 0) ty.
     Proof. Admitted.
 
-    Lemma tm_subst_gen_preservation :
-      forall G1 G2 t ty t' ty',
-        ok_term (G1 ++ Bvar ty' :: G2) t ty ->
-        ok_term (G1 ++ G2) t' ty' ->
-        ok_term (G1 ++ G2) (tm_subst_gen t (length (vars G1)) t') ty.
-    Proof.
-      introv ttype.
-      remember (G1 ++ Bvar ty1 :: G2) as Gamma eqn:HGamma.
-      gen t' ty1 G1.
-      induction ttype ; intros ; subst*.
-      { Case "TmVar". with_hyp (Nth _ _ _) as Hvar.
-        unfold tm_subst_gen.
-        lets [ in_vs1 | (m & Heqm & in_vs2') ] : Nth_app_inv Hvar.
-        { lets Hlt : Nth_inbound in_vs1. rewrites (>> If_l Hlt).
-          constructor*. applys* Nth_app_l. }
-        { subst. assert (nlt : ~(length (vars G1) + m < length (vars G1))). nat_math.
-          rewrites* (>> If_r nlt).
-          lets [ (Heq0 & Heq) | (m' & Heqm' & in_vs2) ] : Nth_cons_inv in_vs2' ; subst.
-          { inverts Heq. rewrites* (>> If_l plus_zero_r). }
-          { rew_nat. assert (neq : S (length (vars G1) + m') <> length (vars G1)). nat_math.
-            rewrites (>> If_r neq). rewrite Nat.add_comm.
-            constructor*. applys Nth_app_r in_vs2. } } }
-      { Case "TmLam". constructors*.
-        applys* ok_type_strengthen_vars ty0.
-        applys_eq* (IHttype (tm_shift t') ty0 (Bvar ty1 :: G1)). unfolds* is_var.
-        applys_eq* (ok_term_weaken_vars (G1 ++ G2) ty1). }
-      { Case "TmTyLam". constructors*.
-        applys* ok_kind_strengthen_vars ty1. folds (tm_subst_gen t (length (filter is_var G1)) (tm_ty_shift t')).
-        applys_eq* (IHttype (tm_ty_shift t') (Btvar k :: G1) (ty_shift ty1)).
-        applys* ok_term_tvars_weaken (Gamma <| vars := vs1 ++ vs2 |> <| tvars := tvs |>). }
-      { Case "TmTyApp". constructors*.
-        applys* ok_type_ignores_vars (Gamma <| vars := vs1 ++ ty1 :: vs2 |> <| tvars := tvs |>). }
-    Qed.
+    Lemma open_subst_comm :
+      forall t n t',
+        tm_open (tm_subst t n t') = tm_subst (tm_open t) (S n) (tm_freshen t' 0).
+    (* Needs local closure! *)
+    Proof. Admitted.
+
+    Lemma ok_type_strengthen_var :
+      forall G1 G2 ty' ty k,
+        ok_type (G1 ++ BindVar (Some ty') :: G2) ty k ->
+        ok_type (G1 ++ BindVar None :: G2) ty k.
+    (* Needs local closure! *)
+    Proof. Admitted.
 
     Lemma tm_subst_preservation :
-      forall Gamma t t' ty1 ty2,
-        ok_term (Bvar ty1 :: Gamma) t ty2 ->
-        ok_term Gamma t' ty1 ->
-        ok_term Gamma (tm_subst t t') ty2.
-    Proof. Admitted.
+      forall G1 G2 t t' ty1 ty2,
+        ok_term (G1 ++ BindVar (Some ty1) :: G2) t ty2 ->
+        ok_term (G1 ++ BindVar None :: G2) t' ty1 ->
+        ok_term (G1 ++ BindVar None :: G2) (tm_subst t (length (vars G1)) t') ty2.
+    Proof.
+      introv ttype.
+      remember (G1 ++ BindVar (Some ty1) :: G2) as Gamma eqn:HGamma.
+      gen t' G1.
+      induction ttype ; intros ; subst*.
+      { Case "TmFVar". admit. }
+        (* with_hyp (var_in _ _ _) as Hvar. rew_mcore in Hvar. unfold var_in in Hvar. *)
+        (* unfold tm_subst. *)
+        (* lets [ (Heq0 & Heq) | (m & Heqm & in_Gamma) ] : Nth_cons_inv Hvar ; subst. *)
+        (* { case_if*. inverts* Heq. } *)
+        (* { case_if*. nat_math. rew_nat in *. constructor. unfold var_in. rew_mcore*. } } *)
+      { Case "TmLam". constructor. applys* ok_type_strengthen_var ty1.
+        rewrite open_subst_comm.
+        applys_eq* (IHttype (tm_freshen t' 0) (BindVar (Some ty0) :: G1)). rew_mcore*.
+        rew_list. applys* tm_freshen_preservation. }
+    Admitted.
 
     Lemma tm_ty_subst_preservation :
       forall Gamma t ty ty' k,
-        ok_term (Btvar k :: Gamma) t ty' ->
-        ok_type Gamma ty k ->
-        ok_term Gamma (tm_ty_subst t ty) (ty_subst ty' ty).
+        ok_term (Btvar k :: Gamma) (tm_ty_open t) (ty_open ty) ->
+        ok_type Gamma ty' k ->
+        ok_term Gamma (tm_ty_bsubst t 0 ty') (ty_bsubst ty 0 ty').
     Admitted.
 
     Theorem preservation :
